src/program_proof/memkv/bank_proof.v
@@ -2,7 +2,7 @@ From Perennial.algebra Require Import auth_map.
 From Perennial.program_proof Require Import grove_prelude std_proof.
 From Goose.github_com.mit_pdos.gokv Require Import memkv lockservice bank.
 From Perennial.program_logic Require Import atomic_fupd.
-From Perennial.program_proof.memkv Require Export common_proof urpc_lib memkv_clerk_proof lockservice_proof.
+From Perennial.program_proof.memkv Require Export common_proof erpc_lib memkv_clerk_proof lockservice_proof.
 
 
 Record bank_names := BankNames {
