src/program_proof/memkv/erpc_proof.v
@@ -1,0 +1,44 @@
+From Perennial.Helpers Require Import ModArith.
+From Goose.github_com.mit_pdos.gokv Require Import erpc.
+From Perennial.goose_lang Require Import adequacy.
+From Perennial.base_logic Require Import lib.ghost_map lib.mono_nat lib.saved_spec.
+From Perennial.program_proof Require Import grove_prelude std_proof marshal_stateless_proof.
+From Perennial.program_proof.memkv Require Import urpc_proof urpc_spec erpc_lib.
+
+(** Spec for an eRPC handler.
+This is isomorphic to uRPCSpec, but to avoid confusion we use distinct types. *)
+Record eRPCSpec {Σ} :=
+  { espec_rpcid : u64;
+    espec_ty : Type;
+    espec_Pre : espec_ty → list u8 → iProp Σ;
+    espec_Post : espec_ty → list u8 → list u8 → iProp Σ }.
+
+Section erpc.
+Context `{rpcG Σ (list u8), invGS Σ}.
+
+Local Definition encode_request (rid : RPCRequestID) (payload : list u8) :=
+  u64_le rid.(Req_CID) ++ u64_le rid.(Req_Seq) ++ payload.
+
+(** [Spec] is the spec of the eRPC handler;
+    we compute the spec of the underlying uRPC handler. *)
+Definition eRPCSpec_uRPC γrpc (spec : eRPCSpec (Σ:=Σ)) : uRPCSpec :=
+ {| spec_rpcid := spec.(espec_rpcid);
+    spec_ty := rpc_request_names * RPCRequestID * (list u8) * spec.(espec_ty);
+    spec_Pre :=(λ '(γreq, rid, payload, x) req,
+                  ⌜req = encode_request rid payload⌝ ∗
+                  is_RPCRequest γrpc γreq
+                     (spec.(espec_Pre) x req)
+                     (spec.(espec_Post) x req)
+                     rid
+             )%I;
+    spec_Post :=(λ '(γreq, rid, payload, x) req rep,
+                (RPCRequestStale γrpc rid ∨
+                 RPCReplyReceipt γrpc rid rep)
+             )%I
+ |}.
+
+(** Convenience function to say that a given rpcid has such a handler *)
+Definition handler_erpc_spec`{!urpcregG Σ, !gooseGlobalGS Σ} Γsrv γrpc (host:u64) (spec : eRPCSpec) :=
+  handler_urpc_spec Γsrv host (eRPCSpec_uRPC γrpc spec).
+
+End erpc.
